LIANG-CHUNG HSIA, HUA-CHIEH LI, ANDWEI-LIANG SUN

$$
|S^{\prime}(\boldsymbol{d},\boldsymbol{t})|=|\boldsymbol{I}|-2+2\left\lfloor\frac{d}{\ell}\right\rfloor-(-1)^{td}\boldsymbol{\lambda}=|\boldsymbol{I}|-2+2\left\lfloor\frac{d}{\ell}\right\rfloor-(-1)^{d}\boldsymbol{\lambda}
$$

ℓ where λ = (1+(−1)ℓ) and note that td ≡ d (mod 2) when ℓ is even as (t, ) = 1. In

particular, |S′(d, t)| is independent on t. Therefore, ⌊ ⌋ )√

$$
|f(\boldsymbol{d})|\leq\boldsymbol{\phi}\left(\frac{\ell}{\boldsymbol{d}}\right)\left(|\boldsymbol{l}|-\boldsymbol{2}+\boldsymbol{2}\left|\frac{\boldsymbol{d}}{\ell}\right|-(-\boldsymbol{1})^{d}\boldsymbol{\lambda}\right)\sqrt{\boldsymbol{q}}
$$

and

$$
\begin{array}{l}{{|N-{\boldsymbol\phi}(\ell)(q+1)|\leq\displaystyle\sum_{d|\ell}|c_{\ell}(d)f(d)|}}\\ {{\leq\displaystyle\sum_{d|\ell}|c_{\ell}(d)|{\boldsymbol\phi}\left(\frac{\ell}{d}\right)\left(|I|-2+2\displaystyle\left\lfloor\frac{d}{\ell}\right\rfloor-(-1)^{d}{\boldsymbol\lambda}\right)\sqrt{q}.}}\end{array}
$$

ℓ ℓ By Lemma 3.2, we have cℓ(d)ϕ( ) = µ( )ϕ(ℓ). By dividing ϕ(ℓ), we obtain ∣∣∣∣ ∣∣∣∣≤∑ ∣∣∣∣µ ( )∣∣∣∣ ( ⌊ ⌋

$$
\left|{\frac{N}{{\boldsymbol\phi}(\ell)}}-\left(\emph{q}+1\right)\right|\leq\sum_{\emph{d}|\ell}\left|{\boldsymbol\mu}\left({\frac{\ell}{\emph{d}}}\right)\right|\left(|{\emph{I}}|-2+2\left|{\frac{d}{\ell}}\right|-(-1)^{d}{\emph{\lambda}}\right){\sqrt{\emph{q}}}.
$$

ℓ ℓ ℓ Note that |µ( )| = 1 if is square-free and |µ( )| = 0 otherwise. Observe that the ℓ number of divisors d in which is square-free is 2ω(ℓ). Moreover,

$$
\begin{array}{l}{{{\displaystyle \sum_{d\mid\ell},}}\,(-1)^{d}{\boldsymbol\lambda}={\bf2}^{{\boldsymbol\omega}(\ell)}{\bf\delta}.}\\ {{\mu({\frac{\ell}{d}})\!\ne\!0}}\end{array}
$$

∣∣∣∣ ∣∣∣∣≤ It follows that )√

$$
\left|\frac{\boldsymbol{N}}{\boldsymbol{\phi}(\ell)}-(q+1)\right|\leq\left(2^{\boldsymbol{o}(\ell)}(\left|\boldsymbol{I}\right|-2-\boldsymbol{\delta})+2\right)\sqrt{q}.
$$

As a consequence, if q+ 1 > (2ω(ℓ)(|I|− 2− δ ) + 2)√q, then we can conclude that √

N > 0. By dividing q and taking square on both sides, the last inequality is equivalent

to

$$
q+2+{\frac{1}{q}}>(2^{{\boldsymbol{o}}(\ell)}(|{\boldsymbol{\mathit{I}}}|-2-{\boldsymbol{\mathit{\delta}}})+2)^{2}=(2^{{\boldsymbol{o}}(\ell)}(\ell-3-{\boldsymbol{\mathit{\delta}}})+2)^{2}.
$$

All terms except on both sides are integers and < 1. The result follows. 5+1= Corollary 4.4. If q is congruent to 1 modulo 5, then g2X5+gY 0 is solvable in Fq for some primitive root g of Fq.

Proof. By Theorem 4.3, the result holds for q≥ 34. For q< 34 and q≡ 1 (mod 5), one has q = 11,16,31. For q = 11, one has g = 7 and 72 · (−1)5+ 7 · (−1)5+ 1 = 0. For

= 1+α and F×16 = 〈α〉. Moreover, α2 · (α2)5+α · q= 16, one has F16 = F2(α) with α

(α2)5+1= 0. For q= 31, one has g= 3 and 32 · (−3)5+3 ·35+1= 0.

6+1= Corollary 4.5. If q is congruent to 1 modulo 6, then g2X6+gY 0 is solvable in Fq for some primitive root g of Fq if and only if q> 13.