LIANG-CHUNG HSIA, HUA-CHIEH LI, ANDWEI-LIANG SUN

$$
\sum_{\stackrel{1\leq j,k\leq\ell-1}{j+k=\ell}}\pmb{\mathcal{X}}(-1)^{j+k}\pmb{\mathcal{X}}(g^{-1})^{(2j+k)\prime}J(\pmb{\mathcal{X}}^{j},\pmb{\mathcal{X}}^{k})=-\sum_{j=1}^{\ell-1}\pmb{\mathcal{X}}(-g^{-\prime})^{j}.
$$

Note that the kernel of χ is L. If −g−t ∈ L, then g−tL = −L. This gives ℓ = |F×q /L| ≤ 2 since g−tL also generates F×q /L as 1≤ t ≤ ℓ and (t, ℓ) = 1. This is not our case and thus χ(−g−t) 6= 1. Hence, ∑ℓ−1j=1 χ(−g−t) =−1 and the result follows.

Now, we are ready to prove our main theorem.

Theorem 4.3. Let q be a power of a prime and let ℓ be a proper divisor of q−1. If

$$
\boldsymbol{q}\ge(2^{\boldsymbol{o}(\ell)}(\ell-3-\boldsymbol{\delta})+2)^{2}-2
$$

where ω(ℓ) is the number of distinct prime divisors of ℓ and

$$
\begin{array}{r}{\boldsymbol{\delta}=\left\{\begin{array}{ll}{1}&{\textit{if}4\mid\ell,}\\ {0}&{\textit{otherwise},}\end{array}\right.}\end{array}
$$

then there is a generator g of F×q such that Ng > 0.

Proof. By Proposition 4.1, it is enough to consider the subsum

$$
N=\sum_{1\leq t\leq\ell,\atop(t,\ell)=1}N_{g^{\prime}}
$$

where g is a fixed generator of F×q . Lemma 4.2 gives that

$$
\begin{array}{rlr}&{}&{\textit{N}=\boldsymbol{\wp}(\ell)(\boldsymbol{q}+1)+\underset{\underset{1\leq j,k\leq\ell-1}{j,k\neq\ell}}{\sum_{\boldsymbol{\mathcal{X}}}}\boldsymbol{\mathcal{X}}(-1)^{j+k}\boldsymbol{\jmath}(\boldsymbol{\mathcal{X}}^{j},\boldsymbol{\mathcal{X}}^{k})\boldsymbol{\imath}(j,k)\quad\mathrm{where}}\\ &{}&{\boldsymbol{\imath}(j,k)=\underset{\underset{(t,\ell)=1}{1\leq t\leq\ell}}{\sum_{\boldsymbol{\mathcal{X}}}}\boldsymbol{\mathcal{X}}(g^{-1})^{(2j+k)t}\mathrm{.}}\end{array}
$$

Note that χ(g−1) = ζℓ is a primitive ℓ-th root of 1. Therefore,

$$
\begin{array}{r}{\varepsilon(\ensuremath{j},\ensuremath{k})=\displaystyle\sum_{\stackrel{1\leq\ensuremath{I}\leq\ell,}{(i,\ell)=1}}\!\!\!\!\boldsymbol{\zeta}_{\ell}^{(2\ensuremath{j}+\ensuremath{k})\!t}=c_{\ell}(2\ensuremath{j}+\ensuremath{k}),}\end{array}
$$

is a Ramanujan’s sum and

$$
N=\pmb{\varphi}(\ell)(q+1)+\sum_{\overset{1\leq j,k\leq\ell-1}{j+k\neq\ell}}\pmb{\chi}(-1)^{j+k}\pmb{J}(\pmb{\chi}^{j},\pmb{\chi}^{k})c_{\ell}(2\pmb{j}+k).
$$

Let I = {1,2, . . . , ℓ− 1} and for positive integer d | ℓ and integer t with 1 ≤ t ≤ ℓ/d such that (t,d/ℓ) = 1, we set

$$
S^{\prime}(d,t)=\{(j,k)\in I\times I\mid2\,j\!+\!k\equiv t\!d\quad(\textrm{mod}\ \ell)\ \textrm{and}\ j\!+\!k\neq\ell\}.
$$