The remaining calculation simply involves taking the first projections,which yields:

$$
\begin{array} { r l r } & { } & { ( \mathrm { p r } _ { 1 } ) _ { * } ( h _ { 1 } - h _ { 2 } ) ^ { l } = \displaystyle \sum _ { a = 0 } ^ { l } ( - 1 ) ^ { l - a } { \binom { l } { a } } h ^ { a } \cdot ( \mathrm { p r } _ { 1 } ) _ { * } \mathrm { p r } _ { 2 } ^ { * } h ^ { l - a } } \\ & { } & { = ( - 1 ) ^ { n } { \binom { l } { l - n } } h ^ { l - n } \cdot d [ X ] . \qquad ( l \geq n ) } \end{array}
$$

By substituting $\mathbb { ( } \bot 5$ into $(  { \mathbb { 1 4 } } )$ we have :

$$
\begin{array} { r } { s ( X , \sigma _ { 2 } ( X ) ) = \displaystyle \sum _ { l = n } ^ { 2 n } ( - 1 ) ^ { n + l } { \binom { l } { n } } \cdot d h ^ { l - n } - \displaystyle \sum _ { l = n } ^ { 2 n } 2 ^ { l } s _ { l - n } ( T _ { X } ) \cap [ X ] } \\ { = \displaystyle \sum _ { i = 0 } ^ { n } ( - 1 ) ^ { i } { \binom { i + n } { n } } \cdot d h ^ { i } - \displaystyle \sum _ { i = 0 } ^ { n } 2 ^ { i + n } s _ { i } ( T _ { X } ) \cap [ X ] . } \end{array}
$$

From equation $\textcircled { | 9 \textcircled { \cdot } }$ ,we obtain:

$$
\begin{array} { l } { { \displaystyle \dot { \mathrm {  ~ V } _ { } ) , X \times \sigma _ { 2 } ( X ) } ) = s ( T _ { X } ) \cap s ( X , \sigma _ { 2 } ( X ) ) } \ ~ } \\ { { \displaystyle ~ = \sum _ { i = 0 } ^ { n } \sum _ { a + b = i } \{ ( - 1 ) ^ { b } \binom { b + n } { n } d h ^ { b } \cdot s _ { a } ( T _ { X } ) \cap [ X ] - 2 ^ { b + n } s _ { a } ( T _ { X } ) s _ { b } ( T _ { X } ) \cap \{ X \} \} } \ ~ } \end{array}
$$

by omitting the pull back $( \Delta ( X ) \to X ) ^ { * }$ . Therefore,we obtain the main formula from equation $( \ k _ { 2 } )$ ,which completes the proof. □

Corollary. The multiplicity of $\sigma _ { 2 } ( X )$ along $X$ is $d - 2 ^ { n }$

Proof. The multiplicity of $\sigma _ { 2 } ( X )$ along $X$ is the coefficient of $[ X ]$ in the class $s ( X , \sigma _ { 2 } ( X ) )$ (cf. Chapter 4.3])

# 5Examples

# 5.1In the case of curves

Consider the case where $C$ is a smooth projective curve. Let $g$ be the genus of a curve $C$ . The degree of each term of Segre class $T _ { C }$ is given by $\deg s _ { 0 } ( T _ { C } ) = d$ and $\deg s _ { 1 } ( T _ { C } ) = 2 g - 2$ .By substituting those terms in the main formula we get :

$$
\deg \sigma _ { 3 } ( C ) = \frac { 1 } { 3 ! } ( d ^ { 3 } - 9 d ^ { 2 } + 2 6 d + 2 4 - 6 d g - 2 4 g )
$$

which can be found in $\boxed { 1 2 }$ Proposition 1].

# 5.2In the case of surfaces

Consider the case where $S$ is a smooth projective surface. Let $K$ be the canonical divisor of $S$ ，let $d = h ^ { 2 }$ ，let $\pi = h \cdot K$ ，let $\kappa = K ^ { 2 }$ ，and let $e = c _ { 2 }$ be the topological Euler characteristic. The total Segre class of the tangent sheaf $T _ { S }$ of $S$ has degree $0$ ， $^ { 1 }$ ， and 2 terms, which are given by:

$$
s _ { 0 } ( T _ { S } ) = [ S ] , \ s _ { 1 } ( T _ { S } ) = K , \ s _ { 2 } ( T _ { S } ) = \kappa - e .
$$

By substituting those terms in the main formula we get :

$$
\deg \sigma _ { 3 } ( S ) = { \frac { 1 } { 3 ! } } ( d ^ { 3 } - 3 0 d ^ { 2 } + 2 2 4 d - 3 d ( 5 \pi + \kappa - e ) + 1 9 2 \pi + 5 6 \kappa - 4 0 e )
$$