where $\zeta _ { n }$ is a primitive $n$ -th root of1 in $\mathbb { C }$ . Studying on cyclotomic polynomials, O. Holder $\mathbb { H } \mathrm { \overleftrightarrow { o l . 3 6 } } \mathbb { I }$ showed that the sum $c _ { n } ( m )$ has a nice closed form in terms of the Euler and Mobius functions.Denote $\varphi$ the Euler's totient function and $\mu$ theMobiusfunction. We present it in the following lemma where the right-hand side is also called von Sterneck function $\mathbb { S } ^ { \mathrm { t e O 3 } }$ ï¼ŽA proof is given below to the readers for convenience.For different proofs,one refers to [AA53], [Mol52] and [HW08 Theorem 272].

Lemma 3.2. Let $n \in \mathbb { N }$ and $m \in \mathbb { Z }$ Then

$$
c _ { n } ( m ) = \mu \left( { \frac { n } { ( n , m ) } } \right) { \frac { \varphi ( n ) } { \varphi \left( { \frac { n } { ( n , m ) } } \right) } } .
$$

Proof. First of all,suppose that $m = 1$ . Recall an elementary formula that

$$
\sum _ { k \mid r } \mu ( k ) = { \left\{ \begin{array} { l l } { 1 } & { { \mathrm { i f ~ } } r = 1 ; } \\ { 0 } & { { \mathrm { i f ~ } } r > 0 , } \end{array} \right. }
$$

for $r \in \mathbb { N }$ ([Bur11, Theorem 6.6]). Then

$$
c _ { n } ( 1 ) = \sum _ { t = 1 } ^ { n } \zeta _ { n } ^ { t } \sum _ { k | ( t , n ) } \mu ( k ) = \sum _ { k | n } \mu ( k ) \sum _ { 1 \leq t \leq n , \atop k | ( t , n ) } \zeta _ { n } ^ { t } = \sum _ { k | n } \mu ( k ) \sum _ { 1 \leq t ^ { \prime } \leq { \frac { n } { k } } } ( \zeta _ { n } ^ { k } ) ^ { t ^ { \prime } }
$$

where $\begin{array} { r } { t ^ { \prime } = \frac { t } { k } } \end{array}$ . Since $\zeta _ { n } ^ { k }$ is a primitive $\frac { n } { k }$ -th root of 1, the last sum gives 1 if $k = n$ and O if $k < n$ .Hence, $c _ { n } ( 1 ) = \mu ( n )$

For general $m \in \mathbb { Z }$ , we rewrite $c _ { n } ( m )$ as

$$
c _ { n } ( m ) = \sum _ { t \in ( \mathbb { Z } / n \mathbb { Z } ) ^ { \times } } z ^ { t }
$$

where $z = \zeta _ { n } ^ { m }$ .Let $\begin{array} { r } { d = \frac { n } { ( n , m ) } } \end{array}$ Recall that $( \mathbb { Z } / n \mathbb { Z } ) ^ { \times } = M \cdot N$ where $M$ and $N$ are given in Lemma $| 3 . 1 | .$ Note that $z = \zeta _ { n } ^ { m }$ is a primitive $d$ -th root of 1 since $\begin{array} { r } { \left( d , \frac { m } { ( n , m ) } \right) = 1 } \end{array}$ .Hence,

$$
c _ { n } ( m ) = \sum _ { t _ { 1 } \in M } \sum _ { t _ { 2 } \in N } z ^ { t _ { 1 } t _ { 2 } } = \sum _ { t _ { 1 } \in M } | N | z ^ { t _ { 1 } } = | N | c _ { d } ( 1 ) .
$$

Now, the result follows from $\begin{array} { r } { | N | = \frac { \varphi ( n ) } { \varphi ( d ) } } \end{array}$ and $c _ { d } ( 1 ) = \mu ( d )$ by the first paragraph.

Note that $( n , m ) = ( n , ( n , m ) )$ . Thus, we have the following immediate consequence.

Corollary 3.3. Let $n \in \mathbb { N }$ and $m \in \mathbb { Z }$ Then $c _ { n } ( m ) = c _ { n } ( ( n , m ) )$

As a consequence, we note that if $m ^ { \prime }$ is an integer such that $m ^ { \prime } \equiv m { \pmod { n } }$ ,then we conclude from Corollary $\overline { { \left[ 3 . 3 \right] } }$ that $c _ { n } ( m ^ { \prime } ) = c _ { n } ( m )$

The following decomposition of a Cartesian product is useful for counting pairs of integers. Roughly speaking, the product below is partitioned by parallel lines on $\mathbb { Z } \times \mathbb { Z }$

Lemma 3.4. Let $n \in \mathbb { N }$ and let $I = \{ 1 , 2 , \ldots , n - 1 \}$ .For every $a , b \in \mathbb { Z }$ ,we have

$$
I \times I =  { \downarrow \atop { d \mid n \ 1 \leq t \leq \frac { n } { d } }  } _ { ( t , \frac { n } { d } ) = 1 } \{ ( x , y ) \in I \times I \ \middle | \ a x + b y \equiv t d \quad ( \mathrm { m o d \ } n ) \} .
$$