By omitting pairs $( j , k )$ of $I \times I$ satisfying $j + k = \ell$ ,Lemma $\overline { { 3 . 4 } }$ gives that

$$
N - \varphi ( \ell ) ( q + 1 ) = \sum _ { d | \ell } \sum _ { 1 \leq t \leq \frac { \ell } { d } , \atop ( t , \frac { \ell } { d } ) = 1 } \sum _ { ( j , k ) \in S ^ { \prime } ( d , t ) \atop ( t , \frac { \ell } { d } ) = 1 } \chi ( - 1 ) ^ { j + k } J ( \chi ^ { j } , \chi ^ { k } ) c _ { \ell } ( 2 j + k ) .
$$

For $( j , k ) \in S ^ { \prime } ( d , t )$ ,one has $( 2 j + k , \ell ) = d$ and then $c _ { \ell } ( 2 j + k ) = c _ { \ell } ( d )$ by Corollary3.3] Thus,

$$
N - \varphi ( \ell ) ( q + 1 ) = \sum _ { d | \ell } c _ { \ell } ( d ) f ( d )
$$

where

$$
f ( d ) = \sum _ { \stackrel { 1 \leq t \leq \frac { \ell } { d } } { ( t , \frac { \ell } { d } ) = 1 } } \sum _ { ( j , k ) \in S ^ { \prime } ( d , t ) } \chi ( - 1 ) ^ { j + k } J ( \chi ^ { j } , \chi ^ { k } ) .
$$

We need to estimate $| f ( d ) |$

By definition, every pair $( j , k )$ of $S ^ { \prime } ( d , t )$ satisfies $j + k \not \equiv 0$ (mod $\ell$ and thus $| J ( \chi ^ { j } , \chi ^ { k } ) | =$ $\sqrt { q }$ by (v) of Lemma $\boxed { 2 . 2 }$ Since $| \chi ( - 1 ) | = 1$ , it follows that

$$
\vert f ( d ) \vert \leq \sum _ { \begin{array} { c } { 1 \leq t \leq \frac { \ell } { d } , } \\ { ( t , \frac { \ell } { d } ) = 1 } \end{array} } \vert S ^ { \prime } ( d , t ) \vert \sqrt { q } .
$$

Now, we compute $\left| S ^ { \prime } ( d , t ) \right|$ . Observe that every pair $( j , k )$ in $S ^ { \prime } ( d , t )$ is determined by （ $j \in I$ with the proviso that $j + k \neq \ell$ .Thus,for $( j , k ) \in I \times I$ satisfying the congruence $2 j + k \equiv t d$ (mod e） we have to exclude the pair $( j , k )$ with $j \equiv t d$ (mod e). Note that $t d \leq \ell$ while $j \le \ell - 1$ , this congruence can occur only when $d \not \ni q$ and $j = t d$ .Moreover, as $k \neq 0$ , we also need to exclude the case where $2 j \equiv t d { \mathrm { ~ ( m o d ~ } } \ell { \mathrm { ) } }$ . This depends on the parity of $\ell$ . We discuss in the next paragraph to steer clear of confusing.

Suppose that $\ell$ is odd. Let $s \in I$ be such that $2 s \equiv 1 { \pmod { \ell } }$ . Then, we need to exclude $j \in I$ such that $j \equiv s t d \ ( \mathrm { m o d } \ \ell )$ .If $d = \ell$ ,then there is no such $j$ because $j \not \equiv 0$ (mod $\ell$ ） When $d \not \ni q$ ,there is exactly one $j _ { 0 } \in I$ satisfying $j _ { 0 } \equiv s t d$ (mod e). Remember that we also have to exclude the case where $j = t d$ .As a consequence,if $\ell$ is odd,then

$$
| S ^ { \prime } ( d , t ) | = { \left\{ \begin{array} { l l } { | I | } & { { \mathrm { i f ~ } } d = \ell ; } \\ { | I | - 2 } & { { \mathrm { i f ~ } } d \neq \ell . } \end{array} \right. }
$$

Now we assume that $\ell$ is even. There are three cases to consider: (i) $^ { t d }$ is odd, (ii) td is even and $d \not \ni q$ and (ii) $ t = 1 , d = \ell$ .For case (i),since $t d$ is odd, there is no $j$ such that $2 j \equiv t d$ (mod e). Only the case where $j = t d$ has to be excluded.For (ii) and (ii), we have that $t d$ is even and then there is some $j _ { 1 } \in I$ such that $2 j _ { 1 } \equiv t d$ (mod $\ell$ ).In fact, we have $\begin{array} { r } { j _ { 1 } \equiv \frac { t d } { 2 } } \end{array}$ $( \mathrm { m o d } ~ \frac { \ell } { 2 } )$ .If $d \not \ni q$ ,then either $\begin{array} { r } { j _ { 1 } = \frac { t d } { 2 } } \end{array}$ or $\begin{array} { r } { j _ { 1 } = \frac { t d } { 2 } + \frac { \ell } { 2 } } \end{array}$ and in particular, $j _ { 1 } \neq t d$ in this case. If $d = \ell$ ,then $t = 1$ and $j _ { 1 } = \frac { \ell } { 2 }$ .We conclude that

$$
| S ^ { \prime } ( d , t ) | = \left\{ \begin{array} { l l } { { | I | - 1 } } & { { \mathrm { i f } d = \ell ; } } \\ { { | I | - 1 } } & { { \mathrm { i f } d \ne \ell \mathrm { a n d } t d \mathrm { i s } \mathrm { o d d } ; } } \\ { { | I | - 3 } } & { { \mathrm { o t h e r w i s e } . } } \end{array} \right.
$$