Proof.Let $a , b \in \mathbb { Z }$ be two fixed integers and let

$$
S ( d , t ) = \{ ( x , y ) \in I \times I \mid a x + b y \equiv t d { \pmod { n } } \} .
$$

Then the union of $S ( d , t )$ for all such $d$ and $t$ isa subset of $I \times I$ .This union indeed contains all elements of $I \times I$ To see this,let $( x , y ) \in I \times I$ and let $d = ( a x + b y , n )$ . Pick $1 \leq t \leq \frac { n } { d }$ such that $\textstyle t \equiv { \frac { a x + b y } { d } }$ (mod $\frac { n } { d }$ ).Then $( t , \frac { n } { d } ) = 1$ and $a x + b y \equiv t d { \pmod { n } }$ Thus, $( x , y ) \in S ( d , t )$ .Finally, if $S ( d , t ) \cap S ( d ^ { \prime } , t ^ { \prime } ) \neq \emptyset$ , then choose one pair $( x , y )$ in this intersection. We obtain $d = ( a x + b y , n ) = d ^ { \prime }$ Furthermore, $t d \equiv t ^ { \prime } d { \pmod { n } }$ implies that $t \equiv t ^ { \prime } { \pmod { \frac { n } { d } } }$ .Since $1 \leq t , t ^ { \prime } \leq \frac { n } { d }$ ,we have $t = t ^ { \prime }$ □

# 4.PROOFOFTHEMAINRESULT

Recall that we aim at showing the following sum

$$
N ( q , \ell ) = \sum _ { \stackrel { 1 \leq t \leq q - 1 } { ( t , q - 1 ) = 1 } } N _ { g ^ { t } }
$$

is not equal to zero where $g$ is a fixed generator of $\mathbb { F } _ { q } ^ { \times }$ . It's not hard to see that if $g ^ { t } L = g ^ { s } L$ then $N _ { g ^ { t } } = N _ { g ^ { s } }$ . We have the following reduction for $N ( q , \ell )$

Proposition 4.1. Let $g$ be generator of $\mathbb { F } _ { q } ^ { \times }$ and $\ell \mid q - 1$ Then

$$
N ( q , \ell ) = \frac { \varphi ( q - 1 ) } { \varphi ( \ell ) } \sum _ { 1 \leq t \leq \ell , \atop ( t , \ell ) = 1 } N _ { g ^ { t } } .
$$

Proof.By the definition of $N ( q , \ell )$ ,it is a sum indexed by all elements of $( \mathbb { Z } / ( q - 1 ) \mathbb { Z } ) ^ { \times }$ Recall that $( \mathbb { Z } / ( q - 1 ) \mathbb { Z } ) ^ { \times } = M \cdot N$ where $M$ and $N$ are given in Lemma $\boxed { 3 . 1 }$ for $n = q - 1$ and $d = \ell$ .Note that if $t _ { 1 } \in N$ ,then $t _ { 1 } \equiv 1 { \pmod { \ell } }$ and $g ^ { t _ { 1 } } L = g L$ . It follows that $N _ { g ^ { t _ { 1 } t _ { 2 } } } =$ $N _ { g ^ { t _ { 2 } } }$ for any integer $t _ { 2 }$ .Hence,

$$
N ( q , \ell ) = \sum _ { t \in ( \mathbb { Z } / ( q - 1 ) \mathbb { Z } ) ^ { \times } } N _ { g ^ { t } } = \sum _ { t _ { 1 } \in N } \sum _ { t _ { 2 } \in M } N _ { g ^ { t _ { 1 } t _ { 2 } } } = | N | \sum _ { t _ { 2 } \in M } N _ { g ^ { t _ { 2 } } } .
$$

The result follows since|N|=@-1) and $M \simeq ( \mathbb { Z } / \ell \mathbb { Z } ) ^ { \times }$

Recall from $( 5 )$ that

$$
N _ { g ^ { t } } = q + \sum _ { 1 \leq j , k \leq \ell - 1 } \chi ^ { j } ( - g ^ { - 2 t } ) \chi ^ { k } ( - g ^ { - t } ) J ( \chi ^ { j } , \chi ^ { k } )
$$

where $\chi$ is a nontrivial character of $\mathbb { F } _ { q }$ of order $\ell$ . We can rewrite $N _ { g ^ { t } }$ as follows.

Lemma 4.2. For $1 \leq t \leq \ell$ and $( t , \ell ) = 1$ ，

$$
N _ { g ^ { t } } = q + 1 + \sum _ { { 1 \leq j , k \leq \ell - 1 } , \atop { j + k \neq \ell } } \chi ( - 1 ) ^ { j + k } \chi ( g ^ { - 1 } ) ^ { ( 2 j + k ) t } J ( \chi ^ { j } , \chi ^ { k } ) .
$$