Proof. If $\boldsymbol { j } + \boldsymbol { k } = \boldsymbol { \ell }$ ,then $J ( \chi ^ { j } , \chi ^ { k } ) = - \chi ( - 1 ) ^ { j }$ by (iv) of Lemma $\left[ 2 . 2 \right]$ It follows that

$$
\sum _ { 1 \le j , k \le \ell - 1 , \atop j + k = \ell } \chi ( - 1 ) ^ { j + k } \chi ( g ^ { - 1 } ) ^ { ( 2 j + k ) t } J ( \chi ^ { j } , \chi ^ { k } ) = - \sum _ { j = 1 } ^ { \ell - 1 } \chi ( - g ^ { - t } ) ^ { j } .
$$

Note that the kernel of $\chi$ is $L$ If $- g ^ { - t } \in L$ ,then $g ^ { - t } L = - L$ This gives $\ell = | \mathbb { F } _ { q } ^ { \times } / L | \leq 2$ since $g ^ { - t } L$ also generates $\mathbb { F } _ { q } ^ { \times } / L$ as $1 \leq t \leq \ell$ and $( t , \ell ) = 1$ . This is not our case and thus $\chi ( - g ^ { - t } ) \neq 1$ .Hence, $\begin{array} { r } { \sum _ { j = 1 } ^ { \ell - 1 } \chi ( - g ^ { - t } ) ^ { j } = - 1 } \end{array}$ and the result follows. â–¡

Now, we are ready to prove our main theorem.

Theorem 4.3. Let q be a power of a prime and let $\ell$ be a proper divisor of $q - 1$ f

$$
q \geq ( 2 ^ { \omega ( \ell ) } ( \ell - 3 - \delta ) + 2 ) ^ { 2 } - 2
$$

where $\omega ( \ell )$ is the number of distinct prime divisors of $\ell$ and

$$
\delta = { \left\{ \begin{array} { l l } { 1 } & { i f 4 \mid \ell , } \\ { 0 } & { o t h e r w i s e , } \end{array} \right. }
$$

then there is a generator $g$ d $\mathbb { F } _ { q } ^ { \times }$ such that $N _ { g } > 0$

Proof. By Proposition $\boxed { 4 . 1 }$ it is enough to consider the subsum

$$
N = \sum _ { \stackrel { 1 \leq t \leq \ell , \ell } { ( t , \ell ) = 1 } } N _ { g ^ { t } }
$$

where $g$ is a fixed generator of $\mathbb { F } _ { q } ^ { \times }$ . Lemma $\overline { { 4 . 2 } }$ gives that

$$
\begin{array} { l } { { \displaystyle N = \varphi ( \ell ) ( q + 1 ) + \sum _ { \stackrel { 1 \leq j , k \leq \ell - 1 } { j + k \neq \ell } } \chi ( - 1 ) ^ { j + k } J ( \chi ^ { j } , \chi ^ { k } ) z ( j , k ) \quad \mathrm { w h e r e } } } \\ { { \displaystyle z ( j , k ) = \sum _ { 1 \leq t \leq \ell , \atop ( t , \ell ) = 1 } \chi ( g ^ { - 1 } ) ^ { ( 2 j + k ) t } . } } \end{array}
$$

Note that $\chi ( g ^ { - 1 } ) = \zeta _ { \ell }$ is a primitive $\ell$ -th root of1. Therefore,

$$
z ( j , k ) = \sum _ { \stackrel { 1 \leq t \leq \ell , } { ( t , \ell ) = 1 } } \zeta _ { \ell } ^ { ( 2 j + k ) t } = c _ { \ell } ( 2 j + k ) ,
$$

is a Ramanujan's sum and

$$
N = \varphi ( \ell ) ( q + 1 ) + \sum _ { { 1 \leq j , k \leq \ell - 1 } , \atop { j + k \neq \ell } } \chi ( - 1 ) ^ { j + k } J ( \chi ^ { j } , \chi ^ { k } ) c _ { \ell } ( 2 j + k ) .
$$

Let $I = \{ 1 , 2 , \ldots , \ell - 1 \}$ and for positive integer $d \mid \ell$ and integer $t$ with $1 \leq t \leq \ell / d$ such that $( t , d / \ell ) = 1$ , we set

$$
S ^ { \prime } ( d , t ) = \{ ( j , k ) \in I \times I \mid 2 j + k \equiv t d { \pmod { \ell } } { \mathrm { ~ a n d ~ } } j + k \neq \ell \} .
$$