d $\begin{array} { r } { \operatorname* { l i m } _ { t \to 0 ^ { + } } \frac { ( h _ { W _ { t } } - h _ { K } ) ( u ) } { t } = f ( u ) } \end{array}$ $S _ { K }$ $u$ $0$ $\begin{array} { r } { l _ { d } ( u ) = \operatorname* { l i m } _ { t \to 0 ^ { + } } \frac { ( h _ { W _ { t } } - h _ { K } ) ( u ) } { t } } \end{array}$ $u \in \mathbb { S } ^ { n - 1 }$ Notethat (by definitionof $W _ { t }$ ） $l _ { d } ( u ) \leq f ( u )$ ,for all $u$ .Let $U _ { \epsilon } = \{ u \in \mathbb { S } ^ { n - 1 } : l _ { d } ( u ) < f ( u ) - \epsilon \}$ It is enoughtoshowthat $S _ { K } ( U _ { \epsilon } ) = 0$ (forarbitrary $\epsilon > 0$ ）

By Fatou's lemma,

$$
\begin{array} { r l } { \displaystyle \operatorname* { l i m s u p } _ { t \to 0 ^ { + } } \int _ { U _ { \epsilon } } \frac { \displaystyle ( h _ { W _ { t } } - h _ { K } ) ( u ) } { t } d S _ { K } ( u ) \leq \int _ { U _ { \epsilon } } \operatorname* { l i m s u p } _ { t \to 0 ^ { + } } \frac { \displaystyle ( h _ { W _ { t } } - h _ { K } ) ( u ) } { t } d S _ { K } ( u ) } & { } \\ { = \int _ { U _ { \epsilon } } l _ { d } ( u ) d S _ { K } ( u ) } & { } \\ { \leq \int _ { U _ { \epsilon } } f ( u ) d S _ { K } ( u ) - \epsilon S _ { K } ( U _ { \epsilon } ) . } \end{array}
$$

Therefore :

$$
\operatorname* { l i m } _ { t \to 0 ^ { + } } \frac { V _ { 1 } ( t ) - V _ { 0 } } { t } \le \frac { 1 } { n } \int _ { \Omega } f ( u ) d S _ { K } ( u ) - \frac { \epsilon } { n } S _ { K } ( U _ { \epsilon } ) .
$$

It follows from lemma $1$ that $S _ { K } ( U _ { \epsilon } ) = 0$

Similarly, let $\begin{array} { r } { l _ { g } ( u ) = \operatorname* { l i m } _ { t \to 0 ^ { - } } \frac { ( h _ { W _ { t } } - h _ { K } ) ( u ) } { t } } \end{array}$ ， $u \in \mathbb { S } ^ { n - 1 }$ ,so that $l _ { g } ( u ) \geq f ( u )$ for all $u \in \Omega$ ,and let $V _ { \epsilon } = \{ u \in \mathbb { S } ^ { n - 1 } : l _ { g } ( u ) > f ( u ) + \epsilon \}$ .Fix $x _ { 0 } \in i n t ( K )$ ,and let $K ^ { \prime } = K - x _ { 0 }$ .If $| t |$ is small enough,then a translate of $( 1 - C | t | ) K ^ { \prime }$ is contained in $W _ { t }$ ，with $C = ( \operatorname* { m a x } _ { u } | f | ) / ( \operatorname* { m i n } _ { u } h _ { K ^ { \prime } } ) > 0$

$\begin{array} { r } { \frac { ( h _ { W _ { t } } - h _ { K } ) ( u ) } { t } \leq C h _ { K ^ { \prime } } ( u ) } \end{array}$ for all $u \in \mathbb { S } ^ { n - 1 }$ for any $t < 0$ (with $| t |$ smal cmoiab.

$$
\begin{array} { l } { \displaystyle \operatorname* { l i m } _ { t  0 ^ { - } } \frac { V _ { 1 } - V _ { 0 } } { t } = \frac { 1 } { n } \int _ { V _ { \epsilon } } l _ { g } ( u ) d S _ { K } ( u ) + \frac { 1 } { n } \int _ { \Omega \backslash V _ { \epsilon } } l _ { g } ( u ) d S _ { K } ( u ) } \\ { \displaystyle \quad \geq \frac { 1 } { n } \int _ { \Omega } f ( u ) d S _ { K } ( u ) + \frac { \epsilon } { n } S _ { K } ( V _ { \epsilon } ) . } \end{array}
$$

So that $S _ { K } ( V _ { \epsilon } ) = 0$ ,by lemma 1. It follows that $l _ { g } ( u ) = f ( u )$ for $S _ { K }$ -a.e. $u \in \Omega$

# 4.2.Examples when Proposition 1 applies :computations.We review one of the examples listed afterProposition 2.

Let $M$ behalf a Euclidean ball: ${ \cal M } = B _ { 2 } ^ { n } \cap { \cal H } _ { + }$ ，with $H _ { + } = \{ x \in \mathbb { R } ^ { n } : x _ { n } \geq 0 \}$ .Then

$$
\operatorname { I s o p } ( M ) = { \frac { | \partial M | } { n | M | } } = { \frac { 2 | \partial M | } { n \kappa _ { n } } } = { \frac { n \kappa _ { n } } { n \kappa _ { n } } } + { \frac { 2 \kappa _ { n - 1 } } { n \kappa _ { n } } } = 1 + { \frac { 1 } { n W _ { n } } } > 1 .
$$

where $\begin{array} { r } { W _ { n } = \int _ { 0 } ^ { \pi / 2 } ( \cos ( \phi ) ) ^ { n } d \phi } \end{array}$ (recall that $\kappa _ { n } = 2 \kappa _ { n - 1 } W _ { n }$ ）

Let $T = T _ { a }$ be the linear map such that $T e _ { i } = e _ { i }$ when $i \leq n - 1$ ，and $T e _ { n } = a e _ { n }$ .Then $T B _ { 2 } ^ { \prime \iota } = { \mathcal { E } } _ { a }$ is an ellipsoid of volume $a \kappa _ { n }$ . Moreover one may compute its surface area :

$$
| \partial \mathcal { E } _ { a } | = 2 ( n - 1 ) \kappa _ { n - 1 } \int _ { 0 } ^ { \pi / 2 } R _ { \phi } ^ { n - 1 } ( \cos ( \phi ) ) ^ { n - 2 } d \phi = 2 ( n - 1 ) \kappa _ { n - 1 } \int _ { 0 } ^ { \pi / 2 } r _ { \phi } ^ { n - 1 } \frac { d \phi } { \cos ( \phi ) } \cdot
$$

The equation of the surface $\partial \mathcal { E } _ { a }$ s $\begin{array} { r } { r ^ { 2 } + \frac { h ^ { 2 } } { a ^ { 2 } } = 1 } \end{array}$ ，where $h = x _ { n }$ and $r ^ { 2 } = x _ { 1 } ^ { 2 } + \ldots + x _ { n - 1 } ^ { 2 }$ The surface can be layered according to $r = R \cos ( \phi ) \in [ 0 , 1 ]$ ,and one may write $r$ as $r = : \cos ( \psi )$ for some $\psi \in [ 0 , \frac { \pi } { 2 } ]$ Then $\begin{array} { r } { \tan ^ { 2 } ( \psi ) = \frac { 1 - r ^ { 2 } } { r ^ { 2 } } = \frac { 1 } { a ^ { 2 } } \frac { h ^ { 2 } } { r ^ { 2 } } = \frac { 1 } { a ^ { 2 } } \tan ^ { 2 } ( \phi ) } \end{array}$ ,therefore (differentiating) $( 1 + \tan ^ { 2 } ( \psi ) ) d \psi =$ 1(1+tan²（）)dΦ=1(1+a²tan²())dΦ,i.e.dΦ=1+t²tan) $\begin{array} { r } { d \phi = a \frac { 1 + \tan ^ { 2 } ( \psi ) } { 1 + a ^ { 2 } \tan ^ { 2 } ( \psi ) } d \psi = a \frac { 1 } { 1 + ( a ^ { 2 } - 1 ) \sin ^ { 2 } ( \psi ) } d \psi } \end{array}$