Let $\lambda _ { t } = V _ { 1 } ( t ) / V _ { 0 }$ ,and $\mu _ { t } = V _ { n - 1 } ( t ) / V _ { n } ( t )$ (which are both well-defined and positive,as long as $t > t _ { 0 }$ ).Then，using Brunn-Minkowski's inequality :

$$
( V _ { 1 } - V _ { 0 } ) \sum _ { r = 0 } ^ { n - 1 } \lambda _ { t } ^ { r } = { \frac { V _ { 1 } ^ { n } - V _ { 0 } ^ { n } } { V _ { 0 } ^ { n - 1 } } } \geq { \frac { V _ { n } V _ { 0 } ^ { n - 1 } - V _ { 0 } ^ { n } } { V _ { 0 } ^ { n - 1 } } } = V _ { n } - V _ { 0 } .
$$

And symmetrically :

$$
( V _ { n - 1 } - V _ { n } ) \sum _ { r = 0 } ^ { n - 1 } \mu _ { t } ^ { r } = { \frac { V _ { n - 1 } ^ { n } - V _ { n } ^ { n } } { V _ { n } ^ { n - 1 } } } \geq { \frac { V _ { 0 } V _ { n } ^ { n - 1 } - V _ { n } ^ { n } } { V _ { n } ^ { n - 1 } } } = V _ { 0 } - V _ { n } .
$$

Therefore (combining the above two)

$$
V _ { 1 } - V _ { 0 } \geq \alpha _ { t } ( V _ { n } - V _ { n - 1 } ) \quad { \mathrm { w h e r e ~ } } \alpha _ { t } = { \frac { \sum _ { r = 0 } ^ { n - 1 } \mu _ { t } ^ { r } } { \sum _ { r = 0 } ^ { n - 1 } \lambda _ { t } ^ { r } } } .
$$

Since $W _ { t } \to K$ as $t \to 0$ (for the Hausdorff distance),continuity of $V _ { n } ( . )$ implies that $V _ { k } ( t )  V _ { 0 }$ (for all $k \leq n$ )，while (weak) continuity of ( $L \mapsto S _ { L }$ ） implies that $S _ { W _ { t } }  S _ { K }$ (for the weak topology on Radon measures on the sphere). Therefore $\alpha _ { t }  1$ ,while

$$
\begin{array} { c } { \displaystyle \frac { V _ { n } - V _ { n - 1 } } { t } = \frac { 1 } { n } \int _ { \Omega } \frac { ( h _ { W _ { t } } - h _ { K } ) ( u ) } { t } d S _ { W _ { t } } ( u ) } \\ { \displaystyle \qquad = \frac { 1 } { n } \int _ { \Omega } f ( u ) d S _ { W _ { t } } ( u ) \to \frac { 1 } { n } \int _ { \Omega } f ( u ) d S _ { K } ( u ) } \end{array}
$$

where we used that $h _ { W _ { t } } ( u ) = h _ { K } ( u ) + t f ( u )$ for $S _ { W _ { t } }$ -a.e. $u \in \Omega$ .Hence,

$$
\operatorname* { l i m i n f } _ { t \to 0 ^ { + } } \frac { V _ { 1 } - V _ { 0 } } { t } \geq \left( \operatorname* { l i m } _ { t \to 0 ^ { + } } \alpha _ { t } \right) \left( \operatorname* { l i m } _ { t \to 0 ^ { + } } \frac { V _ { n } - V _ { n - 1 } } { t } \right) = \frac { 1 } { n } \int _ { \Omega } f ( u ) d S _ { K } ( u ) .
$$

Similarly, for all $\begin{array} { r } { t _ { 0 } < t < 0 : \frac { V _ { 1 } - V _ { 0 } } { t } \geq \frac { 1 } { n } \int _ { \Omega } f ( u ) d S _ { K } ( u ) } \end{array}$ , while combining BM1 and BM2 yields

$$
\operatorname* { l i m } _ { t \to 0 ^ { + } } \operatorname* { s u p } _ { t } \frac { V _ { 1 } - V _ { 0 } } { t } \leq \left( \operatorname* { l i m } _ { t \to 0 ^ { - } } \alpha _ { t } \right) \left( \operatorname* { l i m } _ { t \to 0 ^ { - } } \frac { V _ { n } - V _ { n - 1 } } { t } \right) = \frac { 1 } { n } \int _ { \Omega } f ( u ) d S _ { K } ( u ) .
$$

We recallthe statement of the (almost-sure) pointwise convergence Lemma 2 (which we used in the proof of Proposition $1$ ),and provide a simple proof here.

Lemma 4. Let $( W _ { t } ) _ { t }$ be Wulff-shape perturbations of a given conver body $K$ ， with respect to $( \Omega , f )$ Then for $S _ { K }$ -almost every $u \in \mathbb { S } ^ { n - 1 }$

$$
\frac { \mathrm { d } h _ { W _ { t } } ( u ) } { \mathrm { d } t } \bigg | _ { t = 0 } = \operatorname* { l i m } _ { t  0 } \frac { h _ { W _ { t } } ( u ) - h _ { K } ( u ) } { t } = f ( u ) .
$$

Proof. First, recall that， for all $u \in \mathbb { S } ^ { n - 1 }$ ，the map ( $t \mapsto h _ { W _ { t } } ( u ) ,$ ）is concave on $] t _ { 0 } , + \infty [$ ，where $t _ { 0 } = t _ { 0 } ( K , \Omega , f ) = \operatorname* { i n f } \{ t \in \mathbb { R } : | W _ { t } | _ { n } > 0 \}$

Indeed, Let $t _ { 0 } < t _ { 1 } < t _ { 2 }$ ，and let $\lambda \in ( 0 , 1 )$ Let $x \in ( 1 - \lambda ) W _ { t _ { 1 } } + \lambda W _ { t _ { 2 } }$ ，and let $u \in \Omega$ Let $x _ { i } \in W _ { t _ { i } }$ ， $i = 1 , 2$ ，such that $x = ( 1 - \lambda ) x _ { 1 } + \lambda x _ { 2 }$ .Denote $t _ { \lambda } : = ( 1 - \lambda ) t _ { 1 } + \lambda t _ { 2 }$ .Then

$$
\langle x , u \rangle = ( 1 - \lambda ) \langle x _ { 1 } , u \rangle + \lambda \langle x _ { 2 } , u \rangle \leq ( 1 - \lambda ) h _ { W _ { t _ { 1 } } } ( u ) + \lambda h _ { W _ { t _ { 2 } } } ( u ) \leq h _ { K } ( u ) + t _ { \lambda } f ( u ) .
$$

As this holds for any $u \in \Omega$ , one concludes that $( 1 - \lambda ) W _ { t _ { 1 } } + \lambda W _ { t _ { 2 } } \subset W _ { t _ { \lambda } }$ ,from which concavity (on the domain $] t _ { 0 } , + \infty [ )$ of $\mathbf { \Omega } ^ { \prime } t \mapsto h _ { W _ { t } } ( u )$ ）,for any fixed $u \in \mathbb { S } ^ { n - 1 }$ ,readily follows.

In particular, for any $u \in \mathbb { S } ^ { n - 1 }$ ,the map $( t \mapsto h _ { W _ { t } } ( u ) )$ is concave on a neighborhood of $t = 0$ ， implying that $\begin{array} { r } { \operatorname* { l i m } _ { t  0 ^ { + } } \frac { ( h _ { W _ { t } } - h _ { K } ) ( u ) } { t } } \end{array}$ (w-hk)(）and limt-0- $\begin{array} { r } { \operatorname* { l i m } _ { t  0 ^ { - } } \frac { ( h _ { W _ { t } } - h _ { K } ) ( u ) } { t } } \end{array}$ (hwt-k)(u),exist for any u ∈ Sn-1. We now explain how to deduce that right and left derivative (at $t = 0$ ）coincide,for $S _ { K }$ -a.e. $u \in \mathbb { S } ^ { n - 1 }$ ,from lemma 1.