Since  $j$  is an affine morphism, there are no higher direct images and we obtain followings :

$$
\mathrm{ch}E_{\mathcal{L}} = \pi_{2*}(\mathrm{ch}(j_{*}\mathcal{O}_{Z_{2}})\pi_{1}^{*}\mathrm{ch}\mathcal{L}\pi_{1}^{*}\mathrm{td}T_{X})
$$

and

$$
\mathrm{ch}j_{*}\mathcal{O}_{Z_{2}} = j_{*}((\mathrm{td}\mathcal{N})^{-1})
$$

by applying the Grothendieck- Riemann- Roch theorem. Note that  $\pi_2\circ j = \rho$

By the projection formula, we have:

$$
\begin{array}{rl} & {\mathrm{ch}E_{\mathcal{L}} = \pi_{2*}(\mathrm{ch}(j_{*}\mathcal{O}_{Z_{2}})\pi_{1}^{*}\mathrm{ch}\mathcal{L}\pi_{1}^{*}\mathrm{td}T_{X})}\\ & {\qquad = \pi_{2*}(j_{*}\mathrm{ch}(\mathrm{td}\mathcal{N})^{-1}\pi_{1}^{*}\mathrm{ch}\mathcal{L}\pi_{1}^{*}\mathrm{td}T_{X})}\\ & {\qquad = (\pi_{2*}\circ j_{*})(\mathrm{ch}(\mathrm{td}\mathcal{N})^{-1}j^{*}\pi_{1}^{*}\mathrm{ch}\mathcal{L}j^{*}\pi_{1}^{*}\mathrm{td}T_{X})}\\ & {\qquad = \rho_{*}((\mathrm{td}\mathcal{N})^{-1}q^{*}\mathrm{ch}\mathcal{L}q^{*}\mathrm{td}T_{X}).} \end{array}
$$

Consider the sheaf sequence

$$
0\to \mathcal{N}^*\to q^*\Omega_X\to \mathcal{O}_E(-E)\to 0
$$

as given in [6] Lemma 2.1]. (Note that the morphism  $q$  in proposition 3.1 and in [6] are different morphisms.) Taking dual of this sequence, we obtain :

$$
0\to q^{*}T_{X}\to \mathcal{N}\to \mathcal{E}xt^{1}(\mathcal{O}_{E}(-E),\mathcal{O}_{Z_{2}})\to 0.
$$

Therefore we have

$$
(\mathrm{td}\mathcal{N})^{-1} = (q^{*}\mathrm{td}T_{X})^{-1}\cdot (\mathrm{td}\mathcal{E}xt^{1}(\mathcal{O}_{E}(-E),\mathcal{O}_{Z_{2}}))^{-1}.
$$

To evaluate  $\mathrm{td}\mathcal{E}xt^{1}(\mathcal{O}_{E}(- E),\mathcal{O}_{Z_{2}})$  , we consider the exact sequence :

$$
0\to \mathcal{O}_{Z_2}(-2E)\to \mathcal{O}_{Z_2}(-E)\to \mathcal{O}_E(-E)\to 0.
$$

Taking the dual of this sequence, we have :

$$
0\to \mathcal{O}_{Z_2}(E)\to \mathcal{O}_{Z_2}(2E)\to \mathcal{E}xt^1 (\mathcal{O}_E(-E),\mathcal{O}_{Z_2})\to 0.
$$

Therefore, we obtain

$$
\mathrm{td}\mathcal{E}xt^{1}(\mathcal{O}_{E}(-E),\mathcal{O}_{Z_{2}}) = \frac{2E}{1 - e^{-2E}} /\frac{E}{1 - e^{-E}} = \frac{2}{1 + e^{-E}}
$$

and

$$
\begin{array}{rl} & {\mathrm{ch}E_{\mathcal{L}} = \rho_{*}\left(q^{*}\mathrm{ch}\mathcal{L}\frac{1 + e^{-E}}{2}\right)}\\ & {\qquad = \rho_{*}\left(\left(1 + \eta^{*}h_{1} + \frac{1}{2!}\eta^{*}h_{1}^{2} + \frac{1}{3!}\eta^{*}h_{1}^{3} + \dots\right)\cdot \left(1 - \frac{1}{2} E + \frac{1}{4} E^{2} - \frac{1}{12} E^{3} + \dots\right)\right)}\\ & {\qquad = \rho_{*}\left(1 + \left(\eta^{*}h_{1} - \frac{1}{2} E\right) + \left(\frac{1}{2}\eta^{*}h_{1}^{2} - \frac{1}{2}\eta^{*}h_{1}\cdot E + \frac{1}{4} E^{2}\right) + \dots\right)}\\ & {\qquad = 2 + (H - \delta) + \left(\frac{1}{2}\rho_{*}\eta^{*}h_{1}^{2} - \frac{1}{2}\rho_{*}(\eta^{*}h_{1}\cdot E) + \frac{1}{4}\rho_{*}E^{2}\right) + \dots .} \end{array}
$$

So we obtain  $c_{1}(E_{\mathcal{L}}) = H - \delta$