The remaining calculation simply involves taking the first projections, which yields:

$$
\begin{array}{c}{(\mathrm{pr}_1)_*(h_1-h_2)^l=\sum_{a=0}^l(-1)^{l-a}\binom{l}{a}h^a\cdot(\mathrm{pr}_1)_*\mathrm{pr}_2^*h^{l-a}}\\{=(-1)^n\binom{l}{l-n}h^{l-n}\cdot d[X],\qquad(l\geq n)}\end{array}
$$

By substituting  $(15)$  into  $(14)$  we have :

$$
\begin{array}{c}{s(X,\sigma_2(X))=\sum_{l=n}^{2n}(-1)^{n+l}\binom{l}{n}\cdot dh^{l-n}-\sum_{l=n}^{2n}2^ls_{l-n}(T_X)\cap[X]}\\{=\sum_{i=0}^{n}(-1)^i\binom{i+n}{n}\cdot dh^i-\sum_{i=0}^{n}2^{i+n}s_a(T_X)\cap[X].}\end{array}
$$

From equation  $(9)$  we obtain:

$$
\begin{array}{l}{X)\times\sigma_{2}(X))=s(T_{X})\cap s(X,\sigma_{2}(X))}\\{=\sum_{i=0}^{n}\sum_{a+b=i}\{(-1)^{b}\binom{b+n}{n}dh^{b}\cdot s_{a}(T_{X})\cap[X]-2^{b+n}s_{a}(T_{X})s_{b}(T_{X})\}}\end{array}
$$

by omitting the pull back  $(\Delta (X)\to X)^{*}$  . Therefore, we obtain the main formula from equation  $(2)$  , which completes the proof.

Corollary. The multiplicity of  $\sigma_{2}(X)$  along  $X$  is  $d - 2^n$

Proof. The multiplicity of  $\sigma_{2}(X)$  along  $X$  is the coefficient of  $[X]$  in the class  $s(X,\sigma_2(X))$  cf.  $\boxed{8}$  Chapter 4.3])

# 5 Examples

# 5.1 In the case of curves

Consider the case where  $C$  is a smooth projective curve. Let  $g$  be the genus of a curve  $C$  . The degree of each term of Segre class  $T_{C}$  is given by  $\deg s_0(T_C) = d$  and  $\deg s_1(T_C) = 2g - 2$  . By substituting those terms in the main formula we get :

$$
\deg \sigma_3(C) = \frac{1}{3!} (d^3 -9d^2 +26d + 24 - 6dg - 24g)
$$

which can be found in [12 Proposition 1].

# 5.2 In the case of surfaces

Consider the case where  $S$  is a smooth projective surface. Let  $K$  be the canonical divisor of  $S$  , let  $d = h^2$  , let  $\pi = h\cdot K$  , let  $\kappa = K^2$  , and let  $e = c_{2}$  be the topological Euler characteristic. The total Segre class of the tangent sheaf  $T_{S}$  of  $S$  has degree  $\mathrm{0}$  , 1, and 2 terms, which are given by:

$$
s_0(T_S) = [S],s_1(T_S) = K,s_2(T_S) = \kappa -e.
$$

By substituting those terms in the main formula we get :

$$
\deg \sigma_3(S) = \frac{1}{3!} (d^3 -30d^2 +224d - 3d(5\pi +\kappa -e) + 192\pi +56\kappa -40e)
$$