In equation (10), it is deduced that

$$
s(Z_2,\mathbb{P}(E_{\mathcal{L}})) = \sum_{i\geq 0}(-1)^i [Z_2]^{i + 1}.
$$

The Chow ring of the projective bundle,  $A^{*}\mathbb{P}(E_{\mathcal{L}})$ , is well- known, but it is simpler to compute the restriction on  $Z_{2}$  rather than on the projective bundle. Therefore, the power of  $[Z_{2}]$  is computed as follows:

$$
[Z_2]^{i + 1} = ([Z_2]|_{Z_2})^i
$$

for  $i\geq 0$ . Additionally, it is straightforward to apply the push- forward  $r_{*}$  on the cycles on  $Z_{2}$ , as the image  $r(Z_{2})$  is  $X$ . Therefore, the equation (10) can be rewritten as:

$$
s(Z_2,\mathbb{P}(E_{\mathcal{L}})) = \sum_{i\geq 0}(-1)^i ([Z_2]|_{Z_2})^i. \tag{11}
$$

To continue, we require an expression of  $[Z_{2}|_{Z_{2}}]$  as a linear combination of generators of the Chow ring  $A^{*}Z_{2}$ .

Proposition 3.2.  $[Z_{2}]|_{Z_{2}} = 2E + \eta^{*}(h_{1} - h_{2})$  in  $A^{1}Z_{2}$  where  $[Z_{2}]$  is a cycle associated to scheme  $Z_{2}$ .

Proof. We denote the canonical divisors of  $X^{[2]}$  and  $Z_{2}$  as  $K_{X^{[2]}}$  and  $K_{Z_{2}}$ , respectively. The ramification divisor of  $\rho$  is  $E$ , so we have

$$
\rho^{*}K_{X^{[2]}} = K_{Z_{2}} - E. \tag{12}
$$

Equation (12) can be found in some literature, or it can be deduced directly from the following exact sequence of sheaves:

$$
0\to \rho^{*}T_{X^{[2]}}^{*}\to T_{Z_{2}}^{*}\to \mathcal{O}_{E}(-E)\to 0.
$$

Let  $\zeta$  be the first Chern class of the tautological line bundle of  $\mathbb{P}(E_{\mathcal{L}})$ . The normal bundle  $N_{Z_{2}}\mathbb{P}(E_{\mathcal{L}})$  is represented by  $\mathcal{O}_{Z_{2}}([Z_{2}])$

$$
c_{1}(\mathcal{O}_{Z_{2}}([Z_{2}])) = K_{Z_{2}} - K_{\mathbb{P}(E_{\mathcal{L}})}|_{Z_{2}}.
$$

In addition, we have the following adjunction formula for the projective bundle:

$$
K_{\mathbb{P}(E_{\mathcal{L}})} = -2\zeta +\pi^{*}c_{1}(E_{\mathcal{L}}) + \pi^{*}K_{X^{[2]}}.
$$

Note that  $(\pi^{*}K_{X^{[2]}})|_{Z_{2}} = \rho^{*}K_{X^{[2]}} = K_{Z_{2}} - E = K_{Z_{2}} - \rho^{*}\delta$ . Then

$$
c_{1}(\mathcal{O}_{Z_{2}}([Z_{2}])) = 2\zeta |_{Z_{2}} - \rho^{*}(H - \delta) + \rho^{*}\delta
$$

by proposition 3.1 Recall that  $c_{1}(\mathcal{O}_{Z_{2}}(Z_{2}) = [Z_{2}]_{Z_{2}}$  and hence we get

$$
[Z_2]|_{Z_2} = 2\zeta |_{Z_2} - \rho^* (H - 2\delta). \tag{13}
$$

We need information about  $\zeta |_{Z_{2}}$ . We know that  $Z_{2}$  is a closed subvariety of  $X\times X^{[2]}\subset \mathbb{P}H^{0}(X,\mathcal{L})\times X^{[2]}$ . Therefore, we can choose a suitable section of  $\zeta |_{Z_{2}}$  whose zero locus is  $(h\times X^{[2]})\cap Z_{2}$ .

Recall that we have an isomorphism  $Z_{2}\cong Bl_{\Delta (X)}(X\times X)$ , which allows us to view  $Z_{2}\subset X\times X^{[2]}\to X$  as equivalent to  $Bl_{\Delta (X)}(X\times X)\to X\times X\to X$ , where the second morphism is  $\mathrm{pr}_1$ . Thus, we obtain  $\zeta |_{Z_{2}} = \eta^{*}h_{1}|_{Z_{2}}$ .

Substituting this result into (13), we find that

$$
[Z_2]|_{Z_2} = 2E + \eta^* (h_1 - h_2).
$$