Proof. Let  $a,b\in \mathbb{Z}$  be two fixed integers and let

$$
S(d,t) = \{(x,y)\in I\times I\mid ax + by\equiv td\pmod {n}\} .
$$

Then the union of  $S(d,t)$  for all such  $d$  and  $t$  is a subset of  $I\times I$  .This union indeed contains all elements of  $I\times I$  . To see this, let  $(x,y)\in I\times I$  and let  $d = (ax + by,n)$  . Pick  $\textstyle 1\leq t\leq \frac{n}{d}$  such that  $\begin{array}{r}t\equiv \frac{ax + by}{d} (\mathrm{mod}\frac{n}{d}) \end{array}$  . Then  $(t,\textstyle {\frac{n}{d}}) = 1$  and  $ax + by\equiv td$  (mod  $n$  Thus,  $(x,y)\in S(d,t)$  . Finally, if  $S(d,t)\cap S(d^{\prime},t^{\prime})\neq \emptyset$  , then choose one pair  $(x,y)$  in this intersection. We obtain  $d = (ax + by,n) = d^{\prime}$  . Furthermore,  $td\equiv t^{\prime}d^{\prime}$  (mod  $n$  ) implies that  $\begin{array}{r}t\equiv t^{\prime}(\mathrm{mod}\frac{n}{d}) \end{array}$  . Since  $\textstyle 1\leq t,t^{\prime}\leq \frac{n}{d}$  , we have  $t = t^\prime$

# 4.PROOF OF THE MAIN RESULT

Recall that we aim at showing the following sum

$$
N(q,\ell) = \sum_{\stackrel{1\leq t\leq q - 1,}{(t,q - 1) = 1}}N_{g^t}
$$

is not equal to zero where  $g$  is a fixed generator of  $\mathbb{F}_q^\times$  . It's not hard to see that if  $g^{t}L = g^{s}L$  then  $N_{g^t} = N_{g^s}$  . We have the following reduction for  $N(q,\ell)$

Proposition 4.1. Let g be generator of  $\mathbb{F}_q^\times$  and  $\ell \mid q - 1$  . Then

$$
N(q,\ell) = \frac{\phi(q - 1)}{\phi(\ell)}\sum_{\stackrel{1\leq t\leq \ell ,}{(t,\ell) = 1}}N_{g^t}.
$$

Proof. By the definition of  $N(q,\ell)$  , it is a sum indexed by all elements of  $(\mathbb{Z} / (q - 1)\mathbb{Z})^{\times}$  Recall that  $(\mathbb{Z} / (q - 1)\mathbb{Z})^{\times} = M\cdot N$  where  $M$  and  $N$  are given in Lemma 3.1 for  $n = q - 1$  and  $d = \ell$  . Note that if  $t_1\in N$  , then  $t_1\equiv 1$  (mod  $\ell$  ) and  $g^{t_1}L = gL$  . It follows that  $N_{g^{1t_2}} =$ $N_{g^t 2}$  for any integer  $t_2$  . Hence,

$$
N(q,\ell) = \sum_{t\in (\mathbb{Z} / (q - 1)\mathbb{Z})^\times}N_{g^t} = \sum_{t_1\in N}\sum_{t_2\in M}N_{g^{t_1t_2}} = |N|\sum_{t_2\in M}N_{g^{t_2}}.
$$

The result follows since  $\begin{array}{r}{|N| = \frac{\phi(q - 1)}{\phi(\ell)}} \end{array}$  and  $M\simeq (\mathbb{Z} / \ell \mathbb{Z})^{\times}$

Recall from  $(5)$  that

$$
N_{g^t} = q + \sum_{1\leq j,k\leq \ell -1}\chi^j (-g^{-2t})\chi^k (-g^{-t})J(\chi^j,\chi^k)
$$

where  $x$  is a nontrivial character of  $\mathbb{F}_q$  of order  $\ell$  . We can rewrite  $N_{g^t}$  as follows.

Lemma 4.2. For  $1\leq t\leq \ell$  and  $(t,\ell) = 1$

$$
N_{g^t} = q + 1 + \sum_{1\leq j,k\leq \ell -1,\atop j + k\neq \ell}\chi (-1)^{j + k}\chi (g^{-1})^{(2j + k)t}J(\chi^j,\chi^k).
$$