We next prove that  $\begin{array}{r}\lim_{t\to 0^{+}}\frac{(h_{W_t} - h_K)(u)}{t} = f(u) \end{array}$  , for  $S_{K}$  - almost every  $u$  (the proof on the left of 0 is similar). Let  $\begin{array}{r}l_d(u) = \lim_{t\to 0^+}\frac{(h_{W_t} - h_K)(u)}{t} \end{array}$  which is well- defined for all  $u\in \mathbb{S}^{n - 1}$  , by concavity. Note that (by definition of  $W_{t}$ $l_{d}(u)\leq f(u)$  , for all  $u$  . Let  $U_{\epsilon} = \{u\in \mathbb{S}^{n - 1}:l_{d}(u)< f(u) - \epsilon \}$  . It is enough to show that  $S_{K}(U_{\epsilon}) = 0$  (for arbitrary  $\epsilon >0$  -

By Fatou's lemma,

$$
\begin{array}{rl} & {\lim_{t\to 0^{+}}\int_{U_{\epsilon}}\frac{(h_{W_t} - h_K)(u)}{t} dS_K(u)\leq \int_{U_{\epsilon}}\lim_{t\to 0^{+}}\frac{(h_{W_t} - h_K)(u)}{t} dS_K(u)}\\ & {\qquad = \int_{U_{\epsilon}}l_d(u)dS_K(u)}\\ & {\qquad \leq \int_{U_{\epsilon}}f(u)dS_K(u) - \epsilon S_K(U_{\epsilon}).} \end{array}
$$

Therefore :

$$
\lim_{t\to 0^{+}}\frac{V_{1}(t) - V_{0}}{t}\leq \frac{1}{n}\int_{\Omega}f(u)dS_{K}(u) - \frac{\epsilon}{n} S_{K}(U_{\epsilon}).
$$

It follows from lemma 1 that  $S_{K}(U_{\epsilon}) = 0$

Similarly, let  $\begin{array}{r}l_g(u) = \lim_{t\to 0^- }\frac{(h_{W_t} - h_K)(u)}{t} \end{array}$ $u\in \mathbb{S}^{n - 1}$  , so that  $l_{g}(u)\geq f(u)$  for all  $u\in \Omega$  , and let  $V_{\epsilon} = \{u\in \mathbb{S}^{n - 1}:l_{g}(u) > f(u) + \epsilon \}$  . Fix  $x_0\in int(K)$  , and let  $K^{\prime} = K - x_{0}$  . If  $|t|$  is small enough, then a translate of  $(1 - C|t|)K^{\prime}$  is contained in  $W_{t}$  , with  $C = (\max_u|f|) / (\min_uh_{K'}) > 0$

In other words,  $\frac{(h_{W_t} - h_K)(u)}{t} \leq Ch_{K'}(u)$  for all  $u \in \mathbb{S}^{n - 1}$ , for any  $t < 0$  (with  $|t|$  small enough). Hence, by dominated convergence,

$$
\begin{array}{rl} & {\lim_{t\to 0^{-}}\frac{V_1 - V_0}{t} = \frac{1}{n}\int_{V_\epsilon}l_g(u)dS_K(u) + \frac{1}{n}\int_{\Omega \backslash V_\epsilon}l_g(u)dS_K(u)}\\ & {\qquad \geq \frac{1}{n}\int_\Omega f(u)dS_K(u) + \frac{\epsilon}{n} S_K(V_\epsilon).} \end{array}
$$

So that  $S_{K}(V_{\epsilon}) = 0$ , by lemma 1. It follows that  $l_g(u) = f(u)$  for  $S_{K}$ - a.e.  $u \in \Omega$

4.2. Examples when Proposition 1 applies: computations. We review one of the examples listed after Proposition 2.

Let  $M$  be half a Euclidean ball :  $M = B_{2}^{n} \cap H_{+}$ , with  $H_{+} = \{x \in \mathbb{R}^{n}: x_{n} \geq 0 \}$ . Then

$$
\mathrm{Isop}(M) = \frac{|\partial M|}{n|M|} = \frac{2|\partial M|}{n\kappa_n} = \frac{n\kappa_n}{n\kappa_n} +\frac{2\kappa_{n - 1}}{n\kappa_n} = 1 + \frac{1}{nW_n} >1.
$$

where  $W_{n} = \int_{0}^{\pi /2} (\cos (\phi))^{n} d\phi$  (recall that  $n_{n} = 2n_{n - 1} W_{n}$ ).

Let  $T = T_{a}$  be the linear map such that  $T e_{1} = e_{i}$  when  $i\leq n - 1$  , and  $T e_{n} = a e_{n}$  . Then  $TB_{2}^{n} = \mathcal{E}_{a}$  is an ellipsoid of volume  $a\kappa_{n}$  . Moreover one may compute its surface area :

$$
|\partial \mathcal{E}_a| = 2(n - 1)\kappa_{n - 1}\int_0^{\pi /2}R_\phi^{n - 1}(\cos (\phi))^{\pi /2}d\phi = 2(n - 1)\kappa_{n - 1}\int_0^{\pi /2}r_\phi^{n - 1}\frac{d\phi}{\cos(\phi)}.
$$

The equation of the surface  $\partial \mathcal{E}_a$  is  $r^2 + \frac{h^2}{a^2} = 1$ , where  $h = x_{n}$ , and  $r^2 = x_1^2 + \ldots + x_{n - 1}^2$ . The surface can be layered according to  $r = R \cos (\phi) \in [0, 1]$ , and one may write  $r$  as  $r = \cos (\psi)$  for some  $\psi \in [0, \frac{\pi}{2} ]$ . Then  $\tan^2 (\psi) = \frac{1 - r^2}{r^2} = \frac{1}{a^2} \frac{h^2}{r^2} = \frac{1}{a^2} \tan^2 (\phi)$ , therefore (differentiating)  $(1 + \tan^2 (\psi)) d\psi = \frac{1}{a} (1 + \tan^2 (\phi)) d\phi = \frac{1}{a} (1 + a^2 \tan^2 (\psi)) d\phi$ , i.e.  $d\phi = a_1 \frac{1 + \tan^2(\psi)}{1 + a^2 \tan^2(\psi)} d\psi = a \frac{1}{1 + (a^2 - 1) \sin^2(\psi)} d\psi$ .

$$
\begin{array}{r}\cos (\phi) = \frac{r}{R} = \frac{r}{(a^2 - (a^2 - 1)r^2)^{1 / 2}} = \frac{\cos(\psi)}{(1 + (a^2 - 1)\sin^2(\psi))^{1 / 2}}. \end{array}
$$